tests/bitvector1/bitvector1_TestDoubleOfInt_var_value3_1.v
@@ -2,17 +2,6 @@
 (* Beware! Only edit allowed sections below    *)
 Require Import ZArith.
 Require Import Rbase.
-Require int.Int.
-Require int.Abs.
-Require int.EuclideanDivision.
-Require real.Real.
-Require real.FromInt.
-Definition implb(x:bool) (y:bool): bool := match (x,
-  y) with
-  | (true, false) => false
-  | (_, _) => true
-  end.
-
 Parameter pow2: Z -> Z.
 
 
@@ -291,20 +280,41 @@ Axiom lsr_to_nat_sub : forall (b:bv) (s:Z), ((0%Z <= s)%Z /\
 Parameter from_int: Z -> bv.
 
 
+Axiom Abs_le : forall (x:Z) (y:Z), ((Zabs x) <= y)%Z <-> (((-y)%Z <= x)%Z /\
+  (x <= y)%Z).
+
+Parameter div: Z -> Z -> Z.
+
+
+Parameter mod1: Z -> Z -> Z.
+
+
+Axiom Div_mod : forall (x:Z) (y:Z), (~ (y = 0%Z)) -> (x = ((y * (div x
+  y))%Z + (mod1 x y))%Z).
+
+Axiom Div_bound : forall (x:Z) (y:Z), ((0%Z <= x)%Z /\ (0%Z <  y)%Z) ->
+  ((0%Z <= (div x y))%Z /\ ((div x y) <= x)%Z).
+
+Axiom Mod_bound : forall (x:Z) (y:Z), (~ (y = 0%Z)) -> ((0%Z <= (mod1 x
+  y))%Z /\ ((mod1 x y) <  (Zabs y))%Z).
+
+Axiom Mod_1 : forall (x:Z), ((mod1 x 1%Z) = 0%Z).
+
+Axiom Div_1 : forall (x:Z), ((div x 1%Z) = x).
+
 Axiom nth_from_int_high_even : forall (n:Z) (i:Z), (((i <  32%Z)%Z /\
-  (0%Z <= i)%Z) /\ ((int.EuclideanDivision.mod1 (int.EuclideanDivision.div n
-  (pow2 i)) 2%Z) = 0%Z)) -> ((nth (from_int n) i) = false).
+  (0%Z <= i)%Z) /\ ((mod1 (div n (pow2 i)) 2%Z) = 0%Z)) -> ((nth (from_int n)
+  i) = false).
 
 Axiom nth_from_int_high_odd : forall (n:Z) (i:Z), (((i <  32%Z)%Z /\
-  (0%Z <= i)%Z) /\
-  ~ ((int.EuclideanDivision.mod1 (int.EuclideanDivision.div n (pow2 i))
-  2%Z) = 0%Z)) -> ((nth (from_int n) i) = true).
+  (0%Z <= i)%Z) /\ ~ ((mod1 (div n (pow2 i)) 2%Z) = 0%Z)) ->
+  ((nth (from_int n) i) = true).
 
-Axiom nth_from_int_low_even : forall (n:Z), ((int.EuclideanDivision.mod1 n
-  2%Z) = 0%Z) -> ((nth (from_int n) 0%Z) = false).
+Axiom nth_from_int_low_even : forall (n:Z), ((mod1 n 2%Z) = 0%Z) ->
+  ((nth (from_int n) 0%Z) = false).
 
-Axiom nth_from_int_low_odd : forall (n:Z), (~ ((int.EuclideanDivision.mod1 n
-  2%Z) = 0%Z)) -> ((nth (from_int n) 0%Z) = true).
+Axiom nth_from_int_low_odd : forall (n:Z), (~ ((mod1 n 2%Z) = 0%Z)) ->
+  ((nth (from_int n) 0%Z) = true).
 
 Axiom pow2i : forall (i:Z), (0%Z <= i)%Z -> ~ ((pow2 i) = 0%Z).
 
@@ -321,42 +331,37 @@ Axiom nth_sign_positive : forall (n:Z), (0%Z <= n)%Z -> ((nth (from_int2c n)
 
 Axiom nth_from_int2c_high_even_positive : forall (n:Z) (i:Z),
   ((0%Z <= n)%Z /\ (((i <  (32%Z - 1%Z)%Z)%Z /\ (0%Z <= i)%Z) /\
-  ((int.EuclideanDivision.mod1 (int.EuclideanDivision.div n (pow2 i))
-  2%Z) = 0%Z))) -> ((nth (from_int2c n) i) = false).
+  ((mod1 (div n (pow2 i)) 2%Z) = 0%Z))) -> ((nth (from_int2c n) i) = false).
 
 Axiom nth_from_int2c_high_odd_positive : forall (n:Z) (i:Z), ((0%Z <= n)%Z /\
-  (((i <  (32%Z - 1%Z)%Z)%Z /\ (0%Z <= i)%Z) /\
-  ~ ((int.EuclideanDivision.mod1 (int.EuclideanDivision.div n (pow2 i))
+  (((i <  (32%Z - 1%Z)%Z)%Z /\ (0%Z <= i)%Z) /\ ~ ((mod1 (div n (pow2 i))
   2%Z) = 0%Z))) -> ((nth (from_int2c n) i) = true).
 
 Axiom nth_from_int2c_low_even_positive : forall (n:Z), ((0%Z <= n)%Z /\
-  ((int.EuclideanDivision.mod1 n 2%Z) = 0%Z)) -> ((nth (from_int2c n)
-  0%Z) = false).
+  ((mod1 n 2%Z) = 0%Z)) -> ((nth (from_int2c n) 0%Z) = false).
 
 Axiom nth_from_int2c_low_odd_positive : forall (n:Z), ((0%Z <= n)%Z /\
-  ~ ((int.EuclideanDivision.mod1 n 2%Z) = 0%Z)) -> ((nth (from_int2c n)
-  0%Z) = true).
+  ~ ((mod1 n 2%Z) = 0%Z)) -> ((nth (from_int2c n) 0%Z) = true).
+
+Axiom nth_from_int2c_0 : forall (i:Z), ((i <  32%Z)%Z /\ (0%Z <= i)%Z) ->
+  ((nth (from_int2c 0%Z) i) = false).
 
 Axiom nth_sign_negative : forall (n:Z), (n <  0%Z)%Z -> ((nth (from_int2c n)
   (32%Z - 1%Z)%Z) = true).
 
 Axiom nth_from_int2c_high_even_negative : forall (n:Z) (i:Z),
   ((n <  0%Z)%Z /\ (((i <  (32%Z - 1%Z)%Z)%Z /\ (0%Z <= i)%Z) /\
-  ((int.EuclideanDivision.mod1 (int.EuclideanDivision.div n (pow2 i))
-  2%Z) = 0%Z))) -> ((nth (from_int2c n) i) = true).
+  ((mod1 (div n (pow2 i)) 2%Z) = 0%Z))) -> ((nth (from_int2c n) i) = true).
 
 Axiom nth_from_int2c_high_odd_negative : forall (n:Z) (i:Z), ((n <  0%Z)%Z /\
-  (((i <  (32%Z - 1%Z)%Z)%Z /\ (0%Z <= i)%Z) /\
-  ~ ((int.EuclideanDivision.mod1 (int.EuclideanDivision.div n (pow2 i))
+  (((i <  (32%Z - 1%Z)%Z)%Z /\ (0%Z <= i)%Z) /\ ~ ((mod1 (div n (pow2 i))
   2%Z) = 0%Z))) -> ((nth (from_int2c n) i) = false).
 
 Axiom nth_from_int2c_low_even_negative : forall (n:Z), ((n <  0%Z)%Z /\
-  ((int.EuclideanDivision.mod1 n 2%Z) = 0%Z)) -> ((nth (from_int2c n)
-  0%Z) = true).
+  ((mod1 n 2%Z) = 0%Z)) -> ((nth (from_int2c n) 0%Z) = true).
 
 Axiom nth_from_int2c_low_odd_negative : forall (n:Z), ((n <  0%Z)%Z /\
-  ~ ((int.EuclideanDivision.mod1 n 2%Z) = 0%Z)) -> ((nth (from_int2c n)
-  0%Z) = false).
+  ~ ((mod1 n 2%Z) = 0%Z)) -> ((nth (from_int2c n) 0%Z) = false).
 
 Parameter bv1 : Type.
 
@@ -499,19 +504,18 @@ Parameter from_int1: Z -> bv1.
 
 
 Axiom nth_from_int_high_even1 : forall (n:Z) (i:Z), (((i <  64%Z)%Z /\
-  (0%Z <= i)%Z) /\ ((int.EuclideanDivision.mod1 (int.EuclideanDivision.div n
-  (pow2 i)) 2%Z) = 0%Z)) -> ((nth1 (from_int1 n) i) = false).
+  (0%Z <= i)%Z) /\ ((mod1 (div n (pow2 i)) 2%Z) = 0%Z)) ->
+  ((nth1 (from_int1 n) i) = false).
 
 Axiom nth_from_int_high_odd1 : forall (n:Z) (i:Z), (((i <  64%Z)%Z /\
-  (0%Z <= i)%Z) /\
-  ~ ((int.EuclideanDivision.mod1 (int.EuclideanDivision.div n (pow2 i))
-  2%Z) = 0%Z)) -> ((nth1 (from_int1 n) i) = true).
+  (0%Z <= i)%Z) /\ ~ ((mod1 (div n (pow2 i)) 2%Z) = 0%Z)) ->
+  ((nth1 (from_int1 n) i) = true).
 
-Axiom nth_from_int_low_even1 : forall (n:Z), ((int.EuclideanDivision.mod1 n
-  2%Z) = 0%Z) -> ((nth1 (from_int1 n) 0%Z) = false).
+Axiom nth_from_int_low_even1 : forall (n:Z), ((mod1 n 2%Z) = 0%Z) ->
+  ((nth1 (from_int1 n) 0%Z) = false).
 
-Axiom nth_from_int_low_odd1 : forall (n:Z), (~ ((int.EuclideanDivision.mod1 n
-  2%Z) = 0%Z)) -> ((nth1 (from_int1 n) 0%Z) = true).
+Axiom nth_from_int_low_odd1 : forall (n:Z), (~ ((mod1 n 2%Z) = 0%Z)) ->
+  ((nth1 (from_int1 n) 0%Z) = true).
 
 Axiom pow2i1 : forall (i:Z), (0%Z <= i)%Z -> ~ ((pow2 i) = 0%Z).
 
@@ -528,42 +532,40 @@ Axiom nth_sign_positive1 : forall (n:Z), (0%Z <= n)%Z ->
 
 Axiom nth_from_int2c_high_even_positive1 : forall (n:Z) (i:Z),
   ((0%Z <= n)%Z /\ (((i <  (64%Z - 1%Z)%Z)%Z /\ (0%Z <= i)%Z) /\
-  ((int.EuclideanDivision.mod1 (int.EuclideanDivision.div n (pow2 i))
-  2%Z) = 0%Z))) -> ((nth1 (from_int2c1 n) i) = false).
+  ((mod1 (div n (pow2 i)) 2%Z) = 0%Z))) -> ((nth1 (from_int2c1 n)
+  i) = false).
 
 Axiom nth_from_int2c_high_odd_positive1 : forall (n:Z) (i:Z),
   ((0%Z <= n)%Z /\ (((i <  (64%Z - 1%Z)%Z)%Z /\ (0%Z <= i)%Z) /\
-  ~ ((int.EuclideanDivision.mod1 (int.EuclideanDivision.div n (pow2 i))
-  2%Z) = 0%Z))) -> ((nth1 (from_int2c1 n) i) = true).
+  ~ ((mod1 (div n (pow2 i)) 2%Z) = 0%Z))) -> ((nth1 (from_int2c1 n)
+  i) = true).
 
 Axiom nth_from_int2c_low_even_positive1 : forall (n:Z), ((0%Z <= n)%Z /\
-  ((int.EuclideanDivision.mod1 n 2%Z) = 0%Z)) -> ((nth1 (from_int2c1 n)
-  0%Z) = false).
+  ((mod1 n 2%Z) = 0%Z)) -> ((nth1 (from_int2c1 n) 0%Z) = false).
 
 Axiom nth_from_int2c_low_odd_positive1 : forall (n:Z), ((0%Z <= n)%Z /\
-  ~ ((int.EuclideanDivision.mod1 n 2%Z) = 0%Z)) -> ((nth1 (from_int2c1 n)
-  0%Z) = true).
+  ~ ((mod1 n 2%Z) = 0%Z)) -> ((nth1 (from_int2c1 n) 0%Z) = true).
+
+Axiom nth_from_int2c_01 : forall (i:Z), ((i <  64%Z)%Z /\ (0%Z <= i)%Z) ->
+  ((nth1 (from_int2c1 0%Z) i) = false).
 
 Axiom nth_sign_negative1 : forall (n:Z), (n <  0%Z)%Z ->
   ((nth1 (from_int2c1 n) (64%Z - 1%Z)%Z) = true).
 
 Axiom nth_from_int2c_high_even_negative1 : forall (n:Z) (i:Z),
   ((n <  0%Z)%Z /\ (((i <  (64%Z - 1%Z)%Z)%Z /\ (0%Z <= i)%Z) /\
-  ((int.EuclideanDivision.mod1 (int.EuclideanDivision.div n (pow2 i))
-  2%Z) = 0%Z))) -> ((nth1 (from_int2c1 n) i) = true).
+  ((mod1 (div n (pow2 i)) 2%Z) = 0%Z))) -> ((nth1 (from_int2c1 n) i) = true).
 
 Axiom nth_from_int2c_high_odd_negative1 : forall (n:Z) (i:Z),
   ((n <  0%Z)%Z /\ (((i <  (64%Z - 1%Z)%Z)%Z /\ (0%Z <= i)%Z) /\
-  ~ ((int.EuclideanDivision.mod1 (int.EuclideanDivision.div n (pow2 i))
-  2%Z) = 0%Z))) -> ((nth1 (from_int2c1 n) i) = false).
+  ~ ((mod1 (div n (pow2 i)) 2%Z) = 0%Z))) -> ((nth1 (from_int2c1 n)
+  i) = false).
 
 Axiom nth_from_int2c_low_even_negative1 : forall (n:Z), ((n <  0%Z)%Z /\
-  ((int.EuclideanDivision.mod1 n 2%Z) = 0%Z)) -> ((nth1 (from_int2c1 n)
-  0%Z) = true).
+  ((mod1 n 2%Z) = 0%Z)) -> ((nth1 (from_int2c1 n) 0%Z) = true).
 
 Axiom nth_from_int2c_low_odd_negative1 : forall (n:Z), ((n <  0%Z)%Z /\
-  ~ ((int.EuclideanDivision.mod1 n 2%Z) = 0%Z)) -> ((nth1 (from_int2c1 n)
-  0%Z) = false).
+  ~ ((mod1 n 2%Z) = 0%Z)) -> ((nth1 (from_int2c1 n) 0%Z) = false).
 
 Parameter concat: bv -> bv -> bv1.
 
@@ -640,6 +642,9 @@ Axiom double_of_bv64_value : forall (b:bv1), ((0%Z <  (to_nat_sub1 b 62%Z
   62%Z 52%Z) - 1023%Z)%Z))%R * (1%R + ((IZR (to_nat_sub1 b 51%Z
   0%Z)) * (pow21 (-52%Z)%Z))%R)%R)%R).
 
+Axiom jp0_30 : forall (i:Z), ((0%Z <= i)%Z /\ (i <  30%Z)%Z) ->
+  ((nth (from_int 2147483648%Z) i) = false).
+
 Axiom nth_const1 : forall (i:Z), ((0%Z <= i)%Z /\ (i <= 30%Z)%Z) ->
   ((nth1 (concat (from_int 1127219200%Z) (from_int 2147483648%Z))
   i) = false).
@@ -710,20 +715,65 @@ Definition var(i:Z): bv1 := (concat (from_int 1127219200%Z) (jpxor i)).
 
 Definition var_as_double(x:Z): R := (double_of_bv64 (var x)).
 
-Axiom nth_var1 : forall (x:bv) (j:Z), ((0%Z <= j)%Z /\ (j <  31%Z)%Z) ->
-  ((nth (bw_xor (from_int 2147483648%Z) x) j) = (nth x j)).
+Definition is_int32(x:Z): Prop := ((-(pow2 31%Z))%Z <= x)%Z /\
+  (x <  (pow2 31%Z))%Z.
 
-Axiom nth_var11 : forall (x:Z) (j:Z), ((0%Z <= j)%Z /\ (j <  31%Z)%Z) ->
-  ((nth1 (var x) j) = (nth (from_int2c x) j)).
+Axiom two_compl_pos : forall (x:Z), ((is_int32 x) /\ (0%Z <= x)%Z) ->
+  ((to_nat_sub (from_int2c x) 31%Z 0%Z) = x).
 
-Axiom nth_var2 : forall (x:Z), ((nth1 (var x)
+Axiom two_compl_neg : forall (x:Z), ((is_int32 x) /\ (x <  0%Z)%Z) ->
+  ((to_nat_sub (from_int2c x) 31%Z 0%Z) = ((pow2 32%Z) + x)%Z).
+
+Axiom nth_0_30 : forall (x:Z), forall (i:Z), ((is_int32 x) /\
+  ((0%Z <= i)%Z /\ (i <= 30%Z)%Z)) -> ((nth (bw_xor (from_int 2147483648%Z)
+  (from_int2c x)) i) = (nth (from_int2c x) i)).
+
+Axiom to_nat_sub_0_30 : forall (x:Z), (is_int32 x) ->
+  ((to_nat_sub (bw_xor (from_int 2147483648%Z) (from_int2c x)) 30%Z
+  0%Z) = (to_nat_sub (from_int2c x) 30%Z 0%Z)).
+
+Axiom jpxorx_pos : forall (x:Z), (0%Z <= x)%Z ->
+  ((nth (bw_xor (from_int 2147483648%Z) (from_int2c x)) 31%Z) = true).
+
+Axiom from_int2c_to_nat_sub : forall (x:Z), (0%Z <= x)%Z ->
+  ((to_nat_sub (from_int2c x) 30%Z 0%Z) = x).
+
+Axiom nth_var31 : forall (x:Z), ((nth (jpxor x)
   31%Z) = (negb (nth (from_int2c x) 31%Z))).
 
-Axiom nth_var30 : forall (x:Z) (k:Z), ((32%Z <= k)%Z /\ (k <= 63%Z)%Z) ->
+Axiom lemma1_pos : forall (x:Z), ((is_int32 x) /\ (0%Z <= x)%Z) ->
+  ((to_nat_sub (jpxor x) 31%Z 0%Z) = ((pow2 31%Z) + x)%Z).
+
+Axiom to_nat_sub_0_30_neg : forall (x:Z), ((is_int32 x) /\ (x <  0%Z)%Z) ->
+  ((to_nat_sub (bw_xor (from_int 2147483648%Z) (from_int2c x)) 30%Z
+  0%Z) = (to_nat_sub (from_int2c x) 30%Z 0%Z)).
+
+Axiom to_nat_sub_0_30_neg1 : forall (x:Z), ((is_int32 x) /\ (x <  0%Z)%Z) ->
+  ((to_nat_sub (from_int2c x) 30%Z 0%Z) = ((pow2 31%Z) + x)%Z).
+
+Axiom lemma1_neg : forall (x:Z), ((is_int32 x) /\ (x <  0%Z)%Z) ->
+  ((to_nat_sub (jpxor x) 31%Z 0%Z) = ((pow2 31%Z) + x)%Z).
+
+Axiom lemma1 : forall (x:Z), (is_int32 x) -> ((to_nat_sub (jpxor x) 31%Z
+  0%Z) = ((pow2 31%Z) + x)%Z).
+
+Axiom nth_var_0_31 : forall (x:Z), forall (i:Z), ((is_int32 x) /\
+  ((0%Z <= i)%Z /\ (i <= 31%Z)%Z)) -> ((nth1 (var x) i) = (nth (jpxor x) i)).
+
+Axiom to_nat_bv32_bv64 : forall (b1:bv), forall (b2:bv),
+  ((to_nat_sub1 (concat b1 b2) 31%Z 0%Z) = (to_nat_sub b2 31%Z 0%Z)).
+
+Axiom to_nat_var_0_31 : forall (x:Z), (is_int32 x) -> ((to_nat_sub1 (var x)
+  31%Z 0%Z) = (to_nat_sub (jpxor x) 31%Z 0%Z)).
+
+Axiom nth_var32to63 : forall (x:Z) (k:Z), ((32%Z <= k)%Z /\ (k <= 63%Z)%Z) ->
   ((nth1 (var x) k) = (nth (from_int 1127219200%Z) (k - 32%Z)%Z)).
 
 Axiom nth_var3 : forall (x:Z), forall (i:Z), ((32%Z <= i)%Z /\
   (i <= 51%Z)%Z) -> ((nth1 (var x) i) = false).
+
+Axiom lemma2 : forall (x:Z), (is_int32 x) -> ((to_nat_sub1 (var x) 51%Z
+  0%Z) = ((pow2 31%Z) + x)%Z).
 
 Axiom nth_var4 : forall (x:Z), forall (i:Z), ((52%Z <= i)%Z /\
   (i <= 53%Z)%Z) -> ((nth1 (var x) i) = true).
@@ -739,68 +789,33 @@ Axiom nth_var7 : forall (x:Z), forall (i:Z), ((58%Z <= i)%Z /\
 
 Axiom nth_var8 : forall (x:Z), ((nth1 (var x) 62%Z) = true).
 
+Axiom lemma3 : forall (x:Z), ((to_nat_sub1 (var x) 62%Z 52%Z) = 1075%Z).
+
 Axiom nth_var9 : forall (x:Z), ((nth1 (var x) 63%Z) = false).
+
+Axiom lemma4 : forall (x:Z), ((nth1 (var x) 63%Z) = false).
 
 Axiom sign_var : forall (x:Z), ((nth1 (var x) 63%Z) = false).
 
-Axiom exp_var : forall (x:Z), ((to_nat_sub1 (var x) 62%Z 52%Z) = 1075%Z).
-
-Axiom to_nat_sub_same : forall (i:bv1), forall (j:bv), forall (m:Z),
-  (forall (k:Z), ((0%Z <= k)%Z /\ (k <= m)%Z) -> ((nth1 i k) = (nth j k))) ->
-  ((to_nat_sub1 i m 0%Z) = (to_nat_sub j m 0%Z)).
-
-Axiom nat_to_sub_x : forall (x:Z), ((to_nat_sub1 (var x) 30%Z
-  0%Z) = (to_nat_sub (from_int2c x) 30%Z 0%Z)).
-
-Axiom to_nat_sub_var : forall (x:Z), ((to_nat_sub1 (var x) 30%Z
-  0%Z) = (to_nat_sub (from_int2c x) 30%Z 0%Z)).
-
-Axiom x_positive : forall (x:Z), ((nth (from_int2c x) 31%Z) = false) ->
-  ((to_nat_sub (from_int2c x) 31%Z 0%Z) = (to_nat_sub (from_int2c x) 30%Z
-  0%Z)).
-
-Axiom sign_of_x : forall (x:Z), ((nth (from_int2c x) 31%Z) = false) ->
-  (0%Z <  x)%Z.
-
-Axiom from_int2c_to_nat_sub : forall (x:Z), (0%Z <  x)%Z ->
-  ((to_nat_sub (from_int2c x) 31%Z 0%Z) = x).
-
-Axiom x_positive1 : forall (x:Z), ((nth (from_int2c x) 31%Z) = false) ->
-  ((to_nat_sub (from_int2c x) 30%Z 0%Z) = x).
-
-Axiom x_positive2 : forall (x:Z), ((nth1 (var x) 31%Z) = true) ->
-  ((to_nat_sub1 (var x) 30%Z 0%Z) = x).
-
-Axiom mantissa_var_x_positive : forall (x:Z), ((nth1 (var x) 31%Z) = true) ->
-  ((to_nat_sub1 (var x) 51%Z 0%Z) = ((pow2 31%Z) + x)%Z).
-
-Axiom x_negative : forall (x:Z), ((nth1 (var x) 31%Z) = false) ->
-  ((to_nat_sub1 (var x) 30%Z 0%Z) = (-x)%Z).
-
-Axiom mantissa_var_x_negative : forall (x:Z), ((nth1 (var x)
-  31%Z) = false) -> ((to_nat_sub1 (var x) 51%Z 0%Z) = ((pow2 31%Z) + x)%Z).
-
-Axiom mantissa_var : forall (x:Z), ((to_nat_sub1 (var x) 51%Z
-  0%Z) = ((pow2 31%Z) + x)%Z).
-
-Axiom var_value0 : forall (x:Z),
+Axiom var_value0 : forall (x:Z), (is_int32 x) ->
   ((var_as_double x) = ((pow21 (1075%Z - 1023%Z)%Z) * (1%R + ((IZR ((pow2 31%Z) + x)%Z) * (pow21 (-52%Z)%Z))%R)%R)%R).
 
-Axiom from_int_sum : forall (x:Z),
+Axiom from_int_sum : forall (x:Z), (is_int32 x) ->
   ((IZR ((pow2 31%Z) + x)%Z) = ((IZR (pow2 31%Z)) + (IZR x))%R).
 
 (* YOU MAY EDIT THE CONTEXT BELOW *)
 Open Scope Z_scope.
 (* DO NOT EDIT BELOW *)
 
-Theorem var_value3 : forall (x:Z),
+Theorem var_value3 : forall (x:Z), (is_int32 x) ->
   ((var_as_double x) = ((pow21 52%Z) + (((pow21 52%Z) * ((IZR (pow2 31%Z)) + (IZR x))%R)%R * (pow21 (-52%Z)%Z))%R)%R).
 (* YOU MAY EDIT THE PROOF BELOW *)
-intro.
+intros.
 rewrite var_value0.
 replace (1075 - 1023) with 52 by omega.
 rewrite plus_IZR.
 ring.
+exact H.
 Qed.
 (* DO NOT EDIT BELOW *)
 
