tests/bitvector1/bitvector1_BitVector_to_nat_of_zero2_2.v
@@ -2,12 +2,6 @@
 (* Beware! Only edit allowed sections below    *)
 Require Import ZArith.
 Require Import Rbase.
-Definition implb(x:bool) (y:bool): bool := match (x,
-  y) with
-  | (true, false) => false
-  | (_, _) => true
-  end.
-
 Parameter pow2: Z -> Z.
 
 
@@ -252,12 +246,12 @@ Axiom lsl_nth_low : forall (b:bv) (n:Z) (s:Z), ((0%Z <= n)%Z /\
 Parameter to_nat_sub: bv -> Z -> Z -> Z.
 
 
-Axiom to_nat_sub_zero : forall (b:bv) (j:Z) (i:Z), ((0%Z <= i)%Z /\
-  (i <= j)%Z) -> (((nth b j) = false) -> ((to_nat_sub b j i) = (to_nat_sub b
-  (j - 1%Z)%Z i))).
+Axiom to_nat_sub_zero : forall (b:bv) (j:Z) (i:Z), (((0%Z <= i)%Z /\
+  (i <= j)%Z) /\ (j <  size)%Z) -> (((nth b j) = false) -> ((to_nat_sub b j
+  i) = (to_nat_sub b (j - 1%Z)%Z i))).
 
-Axiom to_nat_sub_one : forall (b:bv) (j:Z) (i:Z), ((0%Z <= i)%Z /\
-  (i <= j)%Z) -> (((nth b j) = true) -> ((to_nat_sub b j
+Axiom to_nat_sub_one : forall (b:bv) (j:Z) (i:Z), (((0%Z <= i)%Z /\
+  (i <= j)%Z) /\ (j <  size)%Z) -> (((nth b j) = true) -> ((to_nat_sub b j
   i) = ((pow2 (j - i)%Z) + (to_nat_sub b (j - 1%Z)%Z i))%Z)).
 
 Axiom to_nat_sub_high : forall (b:bv) (j:Z) (i:Z), (j <  i)%Z ->
@@ -267,21 +261,39 @@ Axiom to_nat_sub_high : forall (b:bv) (j:Z) (i:Z), (j <  i)%Z ->
 Open Scope Z_scope.
 (* DO NOT EDIT BELOW *)
 
-Theorem to_nat_of_zero2 : forall (b:bv) (i:Z) (j:Z), ((i <= j)%Z /\
-  (0%Z <= i)%Z) -> ((forall (k:Z), ((k <= j)%Z /\ (i <  k)%Z) -> ((nth b
-  k) = false)) -> ((to_nat_sub b j 0%Z) = (to_nat_sub b i 0%Z))).
+Theorem to_nat_of_zero2 : forall (b:bv) (i:Z) (j:Z), (((j <  size)%Z /\
+  (i <= j)%Z) /\ (0%Z <= i)%Z) -> ((forall (k:Z), ((k <= j)%Z /\
+  (i <  k)%Z) -> ((nth b k) = false)) -> ((to_nat_sub b j
+  0%Z) = (to_nat_sub b i 0%Z))).
 (* YOU MAY EDIT THE PROOF BELOW *)
+
 intros b i j (Hij,Hipos).
+cut (j<size).
+
+apply Zlt_lower_bound_ind with (z:=i)
+ (P:=fun j =>j < size ->
+(forall k : Z, k <= j /\ i < k -> nth b k = false) ->
+to_nat_sub b j 0 = to_nat_sub b i 0); auto.
+
+
+
+(*intros b i j (Hij,Hipos).
 apply Zlt_lower_bound_ind with (z:=i)
  (P:=fun j => 
    (forall k : Z, (k <= j) /\ (i < k) -> nth b k = false) ->
    to_nat_sub b j 0 = to_nat_sub b i 0); auto.
+*)
 intros x Hind Hxi.
 assert (h:(i=x\/i < x)) by omega.
 destruct h.
 subst x; auto.
-intros Hbits.
+intros Hbits Hnth.
 rewrite to_nat_sub_zero; auto with zarith.
+destruct Hij.
+exact H0.
+destruct Hij.
+exact H.
+
 (*
 apply Hind.
 omega.
