tests/bitvector1/bitvector1_TestDoubleOfInt_lemma1_pos_1.v
@@ -343,6 +343,9 @@ Axiom nth_from_int2c_low_even_positive : forall (n:Z), ((0%Z <= n)%Z /\
 Axiom nth_from_int2c_low_odd_positive : forall (n:Z), ((0%Z <= n)%Z /\
   ~ ((mod1 n 2%Z) = 0%Z)) -> ((nth (from_int2c n) 0%Z) = true).
 
+Axiom nth_from_int2c_0 : forall (i:Z), ((i <  32%Z)%Z /\ (0%Z <= i)%Z) ->
+  ((nth (from_int2c 0%Z) i) = false).
+
 Axiom nth_sign_negative : forall (n:Z), (n <  0%Z)%Z -> ((nth (from_int2c n)
   (32%Z - 1%Z)%Z) = true).
 
@@ -543,6 +546,9 @@ Axiom nth_from_int2c_low_even_positive1 : forall (n:Z), ((0%Z <= n)%Z /\
 Axiom nth_from_int2c_low_odd_positive1 : forall (n:Z), ((0%Z <= n)%Z /\
   ~ ((mod1 n 2%Z) = 0%Z)) -> ((nth1 (from_int2c1 n) 0%Z) = true).
 
+Axiom nth_from_int2c_01 : forall (i:Z), ((i <  64%Z)%Z /\ (0%Z <= i)%Z) ->
+  ((nth1 (from_int2c1 0%Z) i) = false).
+
 Axiom nth_sign_negative1 : forall (n:Z), (n <  0%Z)%Z ->
   ((nth1 (from_int2c1 n) (64%Z - 1%Z)%Z) = true).
 
@@ -636,6 +642,9 @@ Axiom double_of_bv64_value : forall (b:bv1), ((0%Z <  (to_nat_sub1 b 62%Z
   62%Z 52%Z) - 1023%Z)%Z))%R * (1%R + ((IZR (to_nat_sub1 b 51%Z
   0%Z)) * (pow21 (-52%Z)%Z))%R)%R)%R).
 
+Axiom jp0_30 : forall (i:Z), ((0%Z <= i)%Z /\ (i <  30%Z)%Z) ->
+  ((nth (from_int 2147483648%Z) i) = false).
+
 Axiom nth_const1 : forall (i:Z), ((0%Z <= i)%Z /\ (i <= 30%Z)%Z) ->
   ((nth1 (concat (from_int 1127219200%Z) (from_int 2147483648%Z))
   i) = false).
@@ -715,107 +724,40 @@ Axiom two_compl_pos : forall (x:Z), ((is_int32 x) /\ (0%Z <= x)%Z) ->
 Axiom two_compl_neg : forall (x:Z), ((is_int32 x) /\ (x <  0%Z)%Z) ->
   ((to_nat_sub (from_int2c x) 31%Z 0%Z) = ((pow2 32%Z) + x)%Z).
 
-Axiom lemma1_pos : forall (x:Z), ((is_int32 x) /\ (0%Z <= x)%Z) ->
-  ((to_nat_sub (jpxor x) 31%Z 0%Z) = ((pow2 31%Z) + x)%Z).
+Axiom nth_0_30 : forall (x:Z), forall (i:Z), ((is_int32 x) /\
+  ((0%Z <= i)%Z /\ (i <= 30%Z)%Z)) -> ((nth (bw_xor (from_int 2147483648%Z)
+  (from_int2c x)) i) = (nth (from_int2c x) i)).
 
-Axiom lemma1_neg : forall (x:Z), ((is_int32 x) /\ (x <  0%Z)%Z) ->
-  ((to_nat_sub (jpxor x) 31%Z 0%Z) = ((pow2 31%Z) + x)%Z).
-
-Axiom lemma1 : forall (x:Z), (is_int32 x) -> ((to_nat_sub (jpxor x) 31%Z
-  0%Z) = ((pow2 31%Z) + x)%Z).
-
-Axiom nth_var1 : forall (x:bv) (j:Z), ((0%Z <= j)%Z /\ (j <  31%Z)%Z) ->
-  ((nth (bw_xor (from_int 2147483648%Z) x) j) = (nth x j)).
-
-Axiom nth_var11 : forall (x:Z) (j:Z), ((0%Z <= j)%Z /\ (j <  31%Z)%Z) ->
-  ((nth1 (var x) j) = (nth (from_int2c x) j)).
-
-Axiom nth_var2 : forall (x:Z), ((nth1 (var x)
-  31%Z) = (negb (nth (from_int2c x) 31%Z))).
-
-Axiom nth_var32to63 : forall (x:Z) (k:Z), ((32%Z <= k)%Z /\ (k <= 63%Z)%Z) ->
-  ((nth1 (var x) k) = (nth (from_int 1127219200%Z) (k - 32%Z)%Z)).
-
-Axiom nth_var3 : forall (x:Z), forall (i:Z), ((32%Z <= i)%Z /\
-  (i <= 51%Z)%Z) -> ((nth1 (var x) i) = false).
-
-Axiom lemma2 : forall (x:Z), (is_int32 x) -> ((to_nat_sub1 (var x) 51%Z
-  0%Z) = ((pow2 31%Z) + x)%Z).
-
-Axiom nth_var4 : forall (x:Z), forall (i:Z), ((52%Z <= i)%Z /\
-  (i <= 53%Z)%Z) -> ((nth1 (var x) i) = true).
-
-Axiom nth_var5 : forall (x:Z), forall (i:Z), ((54%Z <= i)%Z /\
-  (i <= 55%Z)%Z) -> ((nth1 (var x) i) = false).
-
-Axiom nth_var6 : forall (x:Z), forall (i:Z), ((56%Z <= i)%Z /\
-  (i <= 57%Z)%Z) -> ((nth1 (var x) i) = true).
-
-Axiom nth_var7 : forall (x:Z), forall (i:Z), ((58%Z <= i)%Z /\
-  (i <= 61%Z)%Z) -> ((nth1 (var x) i) = false).
-
-Axiom nth_var8 : forall (x:Z), ((nth1 (var x) 62%Z) = true).
-
-Axiom lemma3 : forall (x:Z), ((to_nat_sub1 (var x) 62%Z 52%Z) = 1075%Z).
-
-Axiom nth_var9 : forall (x:Z), ((nth1 (var x) 63%Z) = false).
-
-Axiom lemma4 : forall (x:Z), ((nth1 (var x) 63%Z) = false).
-
-Axiom lemma5 : forall (x:Z), (is_int32 x) ->
-  ((var_as_double x) = (((pow21 52%Z) + (pow21 31%Z))%R + (IZR x))%R).
-
-Definition double_of_int32(x:Z): R :=
-  ((var_as_double x) - (double_of_bv64 (concat (from_int 1127219200%Z)
-  (from_int 2147483648%Z))))%R.
-
-Axiom MainResult : forall (x:Z), (is_int32 x) ->
-  ((double_of_int32 x) = (IZR x)).
-
-Axiom sign_var : forall (x:Z), ((nth1 (var x) 63%Z) = false).
-
-Axiom exp_var : forall (x:Z), ((to_nat_sub1 (var x) 62%Z 52%Z) = 1075%Z).
-
-Axiom to_nat_sub_same : forall (i:bv1), forall (j:bv), forall (m:Z),
-  (forall (k:Z), ((0%Z <= k)%Z /\ (k <= m)%Z) -> ((nth1 i k) = (nth j k))) ->
-  ((to_nat_sub1 i m 0%Z) = (to_nat_sub j m 0%Z)).
-
-Axiom nat_to_sub_x : forall (x:Z), ((to_nat_sub1 (var x) 30%Z
+Axiom to_nat_sub_0_30 : forall (x:Z), (is_int32 x) ->
+  ((to_nat_sub (bw_xor (from_int 2147483648%Z) (from_int2c x)) 30%Z
   0%Z) = (to_nat_sub (from_int2c x) 30%Z 0%Z)).
 
-Axiom to_nat_sub_var : forall (x:Z), ((to_nat_sub1 (var x) 30%Z
-  0%Z) = (to_nat_sub (from_int2c x) 30%Z 0%Z)).
-
-Axiom x_positive : forall (x:Z), ((nth (from_int2c x) 31%Z) = false) ->
-  ((to_nat_sub (from_int2c x) 31%Z 0%Z) = (to_nat_sub (from_int2c x) 30%Z
-  0%Z)).
-
-Axiom x_negative : forall (x:Z), ((nth (from_int2c x) 31%Z) = true) ->
-  ((to_nat_sub (from_int2c x) 31%Z
-  0%Z) = ((pow2 31%Z) + (to_nat_sub (from_int2c x) 30%Z 0%Z))%Z).
-
-Axiom sign_of_x : forall (x:Z), ((nth (from_int2c x) 31%Z) = false) ->
-  (0%Z <  x)%Z.
+Axiom jpxorx_pos : forall (x:Z), (0%Z <= x)%Z ->
+  ((nth (bw_xor (from_int 2147483648%Z) (from_int2c x)) 31%Z) = true).
 
 Axiom from_int2c_to_nat_sub : forall (x:Z), (0%Z <= x)%Z ->
-  ((to_nat_sub (from_int2c x) 31%Z 0%Z) = x).
+  ((to_nat_sub (from_int2c x) 30%Z 0%Z) = x).
 
-Axiom from_int2c_to_nat_sub_neg : forall (x:Z), (x <  0%Z)%Z ->
-  ((to_nat_sub (from_int2c x) 31%Z 0%Z) = ((pow2 31%Z) + x)%Z).
+Axiom nth_var31 : forall (x:Z), ((nth (jpxor x)
+  31%Z) = (negb (nth (from_int2c x) 31%Z))).
 
 (* YOU MAY EDIT THE CONTEXT BELOW *)
 Open Scope Z_scope.
 (* DO NOT EDIT BELOW *)
 
-Theorem x_positive1 : forall (x:Z), ((nth (from_int2c x) 31%Z) = false) ->
-  ((to_nat_sub (from_int2c x) 30%Z 0%Z) = x).
+Theorem lemma1_pos : forall (x:Z), ((is_int32 x) /\ (0%Z <= x)%Z) ->
+  ((to_nat_sub (jpxor x) 31%Z 0%Z) = ((pow2 31%Z) + x)%Z).
 (* YOU MAY EDIT THE PROOF BELOW *)
-intros x H.
-rewrite<-x_positive;auto.
-rewrite from_int2c_to_nat_sub;auto.
-apply sign_of_x;exact H.
-
-
+intros.
+unfold jpxor.
+rewrite to_nat_sub_one;auto with zarith.
+replace (31-0) with 31 by omega.
+replace (31-1) with 30 by omega.
+rewrite to_nat_sub_0_30;auto.
+rewrite from_int2c_to_nat_sub;auto with zarith.
+destruct H.
+exact H.
+rewrite jpxorx_pos;auto with zarith.
 Qed.
 (* DO NOT EDIT BELOW *)
 
